<?xml version="1.0" encoding="utf-8"?>
<rdf:RDF xmlns:cc="http://creativecommons.org/ns#"
   xmlns:dc="http://purl.org/dc/elements/1.1/"
   xmlns:lexinfo="http://www.lexinfo.net/ontology/3.0/lexinfo#"
   xmlns:ontolex="http://www.w3.org/ns/lemon/ontolex#"
   xmlns:owl="http://www.w3.org/2002/07/owl#"
   xmlns:rdf="http://www.w3.org/1999/02/22-rdf-syntax-ns#"
   xmlns:rdfs="http://www.w3.org/2000/01/rdf-schema#"
   xmlns:skos="http://www.w3.org/2004/02/skos/core#"
   xmlns:synsem="http://www.w3.org/ns/lemon/synsem#"
   xmlns:vann="http://purl.org/vocab/vann/"
   xmlns:voaf="http://purl.org/vocommons/voaf#"
   xmlns:xsd="http://www.w3.org/2001/XMLSchema#"
   xmlns="https://globalwordnet.github.io/schemas/wn#">
  <voaf:Vocabulary rdf:about="https://globalwordnet.github.io/schemas/wn">
    <cc:attributionName>Global Wordnet Association</cc:attributionName>
    <cc:attributionURL rdf:resource="http://www.globalwordnet.org"/>
    <cc:license rdf:resource="http://creativecommons.org/licenses/by/4.0"/>
    <dc:contributor rdf:resource="http://john.mccr.ae"/>
    <dc:description xml:lang="en">TODO</dc:description>
    <dc:issued rdf:datatype="http://www.w3.org/2001/XMLSchema#date">2014-08-13</dc:issued>
    <dc:modified rdf:datatype="http://www.w3.org/2001/XMLSchema#date">2014-09-13</dc:modified>
    <dc:publisher rdf:resource="http://www.globalwordnet.org"/>
    <dc:rights>Copyright Global Wordnet Association</dc:rights>
    <dc:title xml:lang="en">Global Wordnet RDF Schema</dc:title>
    <vann:preferredNamespacePrefix>wn</vann:preferredNamespacePrefix>
    <vann:preferredNamespaceUri>https://globalwordnet.github.io/schemas/wn#</vann:preferredNamespaceUri>
    <rdf:type rdf:resource="http://www.w3.org/2002/07/owl#Ontology"/>
    <owl:versionInfo xml:lang="en">Development</owl:versionInfo>
  </voaf:Vocabulary>
  <owl:Class rdf:about="https://globalwordnet.github.io/schemas/wn#Count">
    <rdf:label xml:lang="en">count</rdf:label>
  </owl:Class>
  <owl:Class rdf:about="https://globalwordnet.github.io/schemas/wn#Definition">
    <rdfs:label xml:lang="en">definition</rdfs:label>
  </owl:Class>
  <owl:Class rdf:about="https://globalwordnet.github.io/schemas/wn#Example">
    <rdfs:label xml:lang="en">example</rdfs:label>
  </owl:Class>
  <owl:Class rdf:about="https://globalwordnet.github.io/schemas/wn#ILIDefinition">
    <rdfs:label xml:lang="en">ILI definition</rdfs:label>
  </owl:Class>
  <owl:Class rdf:about="https://globalwordnet.github.io/schemas/wn#PartOfSpeech">
    <rdfs:comment xml:lang="en">The syntactic class of the entry, e.g., noun, verb</rdfs:comment>
    <rdfs:label xml:lang="en">part of speech</rdfs:label>
    <rdfs:subClassOf rdf:resource="http://www.lexinfo.net/ontology/3.0/lexinfo#PartOfSpeech"/>
    <owl:oneOf>
      <rdf:Description>
        <rdf:first rdf:resource="https://globalwordnet.github.io/schemas/wn#noun"/>
        <rdf:rest>
          <rdf:Description>
            <rdf:first rdf:resource="https://globalwordnet.github.io/schemas/wn#verb"/>
            <rdf:rest>
              <rdf:Description>
                <rdf:first rdf:resource="https://globalwordnet.github.io/schemas/wn#adjective"/>
                <rdf:rest>
                  <rdf:Description>
                    <rdf:first rdf:resource="https://globalwordnet.github.io/schemas/wn#adverb"/>
                    <rdf:rest>
                      <rdf:Description>
                        <rdf:first rdf:resource="https://globalwordnet.github.io/schemas/wn#adjective_satellite"/>
                        <rdf:rest>
                          <rdf:Description>
                            <rdf:first rdf:resource="https://globalwordnet.github.io/schemas/wn#named_entity"/>
                            <rdf:rest>
                              <rdf:Description>
                                <rdf:first rdf:resource="https://globalwordnet.github.io/schemas/wn#conjunction"/>
                                <rdf:rest>
                                  <rdf:Description>
                                    <rdf:first rdf:resource="https://globalwordnet.github.io/schemas/wn#adposition"/>
                                    <rdf:rest>
                                      <rdf:Description>
                                        <rdf:first rdf:resource="https://globalwordnet.github.io/schemas/wn#other_pos"/>
                                        <rdf:rest>
                                          <rdf:Description>
                                            <rdf:first rdf:resource="https://globalwordnet.github.io/schemas/wn#unknown_pos"/>
                                            <rdf:rest rdf:resource="http://www.w3.org/1999/02/22-rdf-syntax-ns#nil"/>
                                          </rdf:Description>
                                        </rdf:rest>
                                      </rdf:Description>
                                    </rdf:rest>
                                  </rdf:Description>
                                </rdf:rest>
                              </rdf:Description>
                            </rdf:rest>
                          </rdf:Description>
                        </rdf:rest>
                      </rdf:Description>
                    </rdf:rest>
                  </rdf:Description>
                </rdf:rest>
              </rdf:Description>
            </rdf:rest>
          </rdf:Description>
        </rdf:rest>
      </rdf:Description>
    </owl:oneOf>
  </owl:Class>
  <owl:Class rdf:about="https://globalwordnet.github.io/schemas/wn#SenseRelType">
    <rdfs:label xml:lang="en">sense relation type</rdfs:label>
  </owl:Class>
  <owl:Class rdf:about="https://globalwordnet.github.io/schemas/wn#SynsetRelType">
    <rdfs:label xml:lang="en">synset relation type</rdfs:label>
  </owl:Class>
  <owl:Class rdf:about="https://globalwordnet.github.io/schemas/wn#Tag">
    <rdfs:comment xml:lang="en">The tag describing the category of a form</rdfs:comment>
    <rdfs:label xml:lang="en">tag</rdfs:label>
  </owl:Class>
  <PartOfSpeech rdf:about="https://globalwordnet.github.io/schemas/wn#adjective">
    <rdfs:label xml:lang="en">adjective</rdfs:label>
    <owl:sameAs rdf:resource="http://www.lexinfo.net/ontology/3.0/lexinfo#adjective"/>
  </PartOfSpeech>
  <PartOfSpeech rdf:about="https://globalwordnet.github.io/schemas/wn#adjective_satellite">
    <rdfs:label xml:lang="en">adjective satellite</rdfs:label>
  </PartOfSpeech>
  <PartOfSpeech rdf:about="https://globalwordnet.github.io/schemas/wn#adposition">
    <rdfs:label xml:lang="en">adposition</rdfs:label>
    <owl:sameAs rdf:resource="http://www.lexinfo.net/ontology/3.0/lexinfo#adposition"/>
  </PartOfSpeech>
  <PartOfSpeech rdf:about="https://globalwordnet.github.io/schemas/wn#adverb">
    <rdfs:label xml:lang="en">adverb</rdfs:label>
    <owl:sameAs rdf:resource="http://www.lexinfo.net/ontology/3.0/lexinfo#adverb"/>
  </PartOfSpeech>
  <SynsetRelType rdf:about="https://globalwordnet.github.io/schemas/wn#agent">
    <rdf:type rdf:resource="https://globalwordnet.github.io/schemas/wn#SenseRelType"/>
    <rdfs:comment xml:lang="en">A concept which is typically the one/that who/which does the action denoted by a given concept.</rdfs:comment>
    <rdfs:label xml:lang="en">agent</rdfs:label>
    <owl:inverseOf rdf:resource="https://globalwordnet.github.io/schemas/wn#involved_agent"/>
  </SynsetRelType>
  <SynsetRelType rdf:about="https://globalwordnet.github.io/schemas/wn#also">
    <rdf:type rdf:resource="https://globalwordnet.github.io/schemas/wn#SenseRelType"/>
    <rdfs:comment xml:lang="en">a word having a loose semantic relation to another word</rdfs:comment>
    <rdfs:comment xml:lang="ja">当該synsetと相手synsetとの間に何らかの関連がある</rdfs:comment>
    <rdfs:label xml:lang="en">also</rdfs:label>
    <owl:inverseOf rdf:resource="https://globalwordnet.github.io/schemas/wn#also"/>
  </SynsetRelType>
  <SynsetRelType rdf:about="https://globalwordnet.github.io/schemas/wn#anto_converse">
    <rdfs:comment xml:lang="en">word pairs that name or describe a single relationship from opposite perspectives</rdfs:comment>
    <rdfs:label xml:lang="en">converse antonym</rdfs:label>
    <owl:inverseOf rdf:resource="https://globalwordnet.github.io/schemas/wn#anto_converse"/>
  </SynsetRelType>
  <SynsetRelType rdf:about="https://globalwordnet.github.io/schemas/wn#anto_gradable">
    <rdfs:comment xml:lang="en">word pairs whose meanings are opposite and which lie on a continuous spectrum</rdfs:comment>
    <rdfs:label xml:lang="en">gradable antonym</rdfs:label>
    <owl:inverseOf rdf:resource="https://globalwordnet.github.io/schemas/wn#anto_gradable"/>
  </SynsetRelType>
  <SynsetRelType rdf:about="https://globalwordnet.github.io/schemas/wn#anto_simple">
    <rdfs:comment xml:lang="en">word pairs whose meanings are opposite but whose meanings do not lie on a continuous spectrum</rdfs:comment>
    <rdfs:label xml:lang="en">simple antonym</rdfs:label>
    <owl:inverseOf rdf:resource="https://globalwordnet.github.io/schemas/wn#anto_simple"/>
  </SynsetRelType>
  <SynsetRelType rdf:about="https://globalwordnet.github.io/schemas/wn#antonym">
    <rdf:type rdf:resource="https://globalwordnet.github.io/schemas/wn#SenseRelType"/>
    <rdfs:comment xml:lang="en">An opposite and inherently incompatible word</rdfs:comment>
    <rdfs:comment xml:lang="ja">当該語義やsynsetの意味や程度が反対または対の関係となっている語義やsynset</rdfs:comment>
    <rdfs:label xml:lang="en">antonym</rdfs:label>
    <owl:inverseOf rdf:resource="https://globalwordnet.github.io/schemas/wn#antonym"/>
  </SynsetRelType>
  <SynsetRelType rdf:about="https://globalwordnet.github.io/schemas/wn#attribute">
    <rdfs:comment xml:lang="ja">(a=形容詞のsynsetから見て)当該synsetが相手synsetという属性を表す際に使われる
(n=名詞のsynsetから見て)当該synsetという属性を表す際に相手synsetを使う</rdfs:comment>
    <rdfs:comment xml:lang="en">an abstraction belonging to or characteristic of an entity</rdfs:comment>
    <rdfs:label xml:lang="en">attribute</rdfs:label>
    <owl:inverseOf rdf:resource="https://globalwordnet.github.io/schemas/wn#attribute"/>
  </SynsetRelType>
  <owl:DatatypeProperty rdf:about="https://globalwordnet.github.io/schemas/wn#audio">
    <rdfs:comment xml:lang="en">Links to an audio file for a pronunciation</rdfs:comment>
    <rdfs:domain rdf:resource="https://globalwordnet.github.io/schemas/wn#Pronunciation"/>
    <rdfs:label xml:lang="en">audio</rdfs:label>
  </owl:DatatypeProperty>
  <SynsetRelType rdf:about="https://globalwordnet.github.io/schemas/wn#augmentative">
    <rdfs:comment xml:lang="en">A concept used to refer to generally larger members of a class</rdfs:comment>
    <rdfs:label xml:lang="en">augmentative</rdfs:label>
    <owl:inverseOf rdf:resource="https://globalwordnet.github.io/schemas/wn#has_augmentative"/>
  </SynsetRelType>
  <SynsetRelType rdf:about="https://globalwordnet.github.io/schemas/wn#be_in_state">
    <rdfs:comment xml:lang="en">X is qualified by Y</rdfs:comment>
    <rdfs:label xml:lang="en">be in state</rdfs:label>
    <owl:inverseOf rdf:resource="https://globalwordnet.github.io/schemas/wn#state_of"/>
  </SynsetRelType>
  <SynsetRelType rdf:about="https://globalwordnet.github.io/schemas/wn#body_part">
    <rdfs:comment xml:lang="en">A word which is typically a body part of a given word (e.g. "finger")</rdfs:comment>
    <rdfs:label xml:lang="en">body part</rdfs:label>
  </SynsetRelType>
  <SynsetRelType rdf:about="https://globalwordnet.github.io/schemas/wn#by_means_of">
    <rdfs:comment xml:lang="en">A word which is typically the means by which something is done (e.g.,g "deceive" - "deception")</rdfs:comment>
    <rdfs:label xml:lang="en">by means of</rdfs:label>
  </SynsetRelType>
  <owl:DatatypeProperty rdf:about="https://globalwordnet.github.io/schemas/wn#category">
    <rdfs:comment xml:lang="en">The data category of a tag</rdfs:comment>
    <rdfs:domain rdf:resource="https://globalwordnet.github.io/schemas/wn#Tag"/>
    <rdfs:label xml:lang="en">category</rdfs:label>
    <rdfs:range rdf:resource="http://www.w3.org/2001/XMLSchema#string"/>
  </owl:DatatypeProperty>
  <SynsetRelType rdf:about="https://globalwordnet.github.io/schemas/wn#causes">
    <rdfs:comment xml:lang="en">Concept A is an entity that produces an effect or is responsible for events or
results of Concept B.</rdfs:comment>
    <rdfs:comment xml:lang="ja">当該synsetを行うと、相手synsetを引き起こす</rdfs:comment>
    <rdfs:label xml:lang="en">causes</rdfs:label>
    <owl:inverseOf rdf:resource="https://globalwordnet.github.io/schemas/wn#is_caused_by"/>
  </SynsetRelType>
  <SynsetRelType rdf:about="https://globalwordnet.github.io/schemas/wn#classified_by">
    <rdfs:comment xml:lang="en">Concept B is modified by classifier A when it is counted.</rdfs:comment>
    <rdfs:label xml:lang="en">classified by</rdfs:label>
    <owl:inverseOf rdf:resource="https://globalwordnet.github.io/schemas/wn#classifies"/>
  </SynsetRelType>
  <SynsetRelType rdf:about="https://globalwordnet.github.io/schemas/wn#classifies">
    <rdfs:comment xml:lang="en">A concept A used when counting concept B</rdfs:comment>
    <rdfs:label xml:lang="en">classifies</rdfs:label>
    <owl:inverseOf rdf:resource="https://globalwordnet.github.io/schemas/wn#classified_by"/>
  </SynsetRelType>
  <SynsetRelType rdf:about="https://globalwordnet.github.io/schemas/wn#co_agent_instrument">
    <rdfs:comment xml:lang="en">A concept which is the instrument used by a given concept in an action.</rdfs:comment>
    <rdfs:label xml:lang="en">co-agent instrument</rdfs:label>
    <owl:inverseOf rdf:resource="https://globalwordnet.github.io/schemas/wn#co_instrument_agent"/>
  </SynsetRelType>
  <SynsetRelType rdf:about="https://globalwordnet.github.io/schemas/wn#co_agent_patient">
    <rdfs:comment xml:lang="en">A concept which is the patient undergoing an action carried out by a given concept.</rdfs:comment>
    <rdfs:label xml:lang="en">co-agent patient</rdfs:label>
    <owl:inverseOf rdf:resource="https://globalwordnet.github.io/schemas/wn#co_patient_agent"/>
  </SynsetRelType>
  <SynsetRelType rdf:about="https://globalwordnet.github.io/schemas/wn#co_agent_result">
    <rdfs:comment xml:lang="en">A concept which is the result of an action taken by a given concept.</rdfs:comment>
    <rdfs:label xml:lang="en">co-agent result</rdfs:label>
    <owl:inverseOf rdf:resource="https://globalwordnet.github.io/schemas/wn#co_result_agent"/>
  </SynsetRelType>
  <SynsetRelType rdf:about="https://globalwordnet.github.io/schemas/wn#co_instrument_agent">
    <rdfs:comment xml:lang="en">A concept which carries out an action by using a given concept as an instrument.</rdfs:comment>
    <rdfs:label xml:lang="en">co-instrument agent</rdfs:label>
    <owl:inverseOf rdf:resource="https://globalwordnet.github.io/schemas/wn#co_agent_instrument"/>
  </SynsetRelType>
  <SynsetRelType rdf:about="https://globalwordnet.github.io/schemas/wn#co_instrument_patient">
    <rdfs:comment xml:lang="en">A concept which undergoes an action with the use of a given concept as an instrument.</rdfs:comment>
    <rdfs:label xml:lang="en">co-instrument patient</rdfs:label>
    <owl:inverseOf rdf:resource="https://globalwordnet.github.io/schemas/wn#co_patient_instrument"/>
  </SynsetRelType>
  <SynsetRelType rdf:about="https://globalwordnet.github.io/schemas/wn#co_instrument_result">
    <rdfs:comment xml:lang="en">A concept which is the result of an action using an instrument of a given concept.</rdfs:comment>
    <rdfs:label xml:lang="en">co-instrument result</rdfs:label>
    <owl:inverseOf rdf:resource="https://globalwordnet.github.io/schemas/wn#co_result_instrument"/>
  </SynsetRelType>
  <SynsetRelType rdf:about="https://globalwordnet.github.io/schemas/wn#co_patient_agent">
    <rdfs:comment xml:lang="en">A concept which carries out an action a given concept undergoing.</rdfs:comment>
    <rdfs:label xml:lang="en">co-patient agent</rdfs:label>
    <owl:inverseOf rdf:resource="https://globalwordnet.github.io/schemas/wn#co_agent_patient"/>
  </SynsetRelType>
  <SynsetRelType rdf:about="https://globalwordnet.github.io/schemas/wn#co_patient_instrument">
    <rdfs:comment xml:lang="en">A concept which is used as an instrument in an action a given concept undergoes.</rdfs:comment>
    <rdfs:label xml:lang="en">co-patient instrument</rdfs:label>
    <owl:inverseOf rdf:resource="https://globalwordnet.github.io/schemas/wn#co_instrument_patient"/>
  </SynsetRelType>
  <SynsetRelType rdf:about="https://globalwordnet.github.io/schemas/wn#co_result_agent">
    <rdfs:comment xml:lang="en">A concept which takes an action resulting in a given concept.</rdfs:comment>
    <rdfs:label xml:lang="en">co-result agent</rdfs:label>
    <owl:inverseOf rdf:resource="https://globalwordnet.github.io/schemas/wn#co_agent_result"/>
  </SynsetRelType>
  <SynsetRelType rdf:about="https://globalwordnet.github.io/schemas/wn#co_result_instrument">
    <rdfs:comment xml:lang="en">A concept which is used as an instrument in an action resulting in a given concept.</rdfs:comment>
    <rdfs:label xml:lang="en">co-result instrument</rdfs:label>
    <owl:inverseOf rdf:resource="https://globalwordnet.github.io/schemas/wn#co_instrument_result"/>
  </SynsetRelType>
  <SynsetRelType rdf:about="https://globalwordnet.github.io/schemas/wn#co_role">
    <rdfs:comment xml:lang="en">A concept undergoes an action in which a given concept is involved.</rdfs:comment>
    <rdfs:label xml:lang="en">co-role</rdfs:label>
    <owl:inverseOf rdf:resource="https://globalwordnet.github.io/schemas/wn#co_role"/>
  </SynsetRelType>
  <owl:AnnotationProperty rdf:about="https://globalwordnet.github.io/schemas/wn#confidenceScore">
    <rdfs:comment xml:lang="en">A confidence score, usually assigned by an algorithm, with a value between 0 and 1</rdfs:comment>
    <rdfs:label xml:lang="en">confidence score</rdfs:label>
    <rdfs:range rdf:resource="http://www.w3.org/2001/XMLSchema#decimal"/>
  </owl:AnnotationProperty>
  <PartOfSpeech rdf:about="https://globalwordnet.github.io/schemas/wn#conjunction">
    <rdfs:label xml:lang="en">conjunction</rdfs:label>
    <owl:sameAs rdf:resource="http://www.lexinfo.net/ontology/3.0/lexinfo#conjunction"/>
  </PartOfSpeech>
  <owl:ObjectProperty rdf:about="https://globalwordnet.github.io/schemas/wn#count">
    <rdfs:comment xml:lang="en">The count of usages of a sense in some corpus</rdfs:comment>
    <rdfs:domain rdf:resource="http://www.w3.org/ns/lemon/ontolex#LexicalSense"/>
    <rdfs:label xml:lang="en">count</rdfs:label>
    <rdfs:range rdf:resource="https://globalwordnet.github.io/schemas/wn#Count"/>
  </owl:ObjectProperty>
  <owl:ObjectProperty rdf:about="https://globalwordnet.github.io/schemas/wn#definition">
    <rdfs:comment xml:lang="en">A definition of the synset</rdfs:comment>
    <rdfs:domain rdf:resource="http://www.w3.org/ns/lemon/ontolex#LexicalConcept"/>
    <rdfs:label xml:lang="en">definition</rdfs:label>
    <rdfs:range rdf:resource="https://globalwordnet.github.io/schemas/wn#Definition"/>
  </owl:ObjectProperty>
  <SenseRelType rdf:about="https://globalwordnet.github.io/schemas/wn#derivation">
    <rdfs:comment xml:lang="en">A concept which is a derivationally related form of a given concept.</rdfs:comment>
    <rdfs:label xml:lang="en">derivation</rdfs:label>
  </SenseRelType>
  <SynsetRelType rdf:about="https://globalwordnet.github.io/schemas/wn#destination">
    <rdfs:comment xml:lang="en">The noun indicates the destination of a verb (e.g., "retire" - "retiree")</rdfs:comment>
    <rdfs:label xml:lang="en">destination</rdfs:label>
  </SynsetRelType>
  <SynsetRelType rdf:about="https://globalwordnet.github.io/schemas/wn#diminutive">
    <rdfs:comment xml:lang="en">A concept used to refer to generally smaller members of a class</rdfs:comment>
    <rdfs:label xml:lang="en">diminutive</rdfs:label>
    <owl:inverseOf rdf:resource="https://globalwordnet.github.io/schemas/wn#has_diminutive"/>
  </SynsetRelType>
  <SynsetRelType rdf:about="https://globalwordnet.github.io/schemas/wn#direction">
    <rdfs:comment xml:lang="en">A concept which is the direction of the action or event expressed by a given concept.</rdfs:comment>
    <rdfs:label xml:lang="en">direction</rdfs:label>
    <owl:inverseOf rdf:resource="https://globalwordnet.github.io/schemas/wn#involved_direction"/>
  </SynsetRelType>
  <SynsetRelType rdf:about="https://globalwordnet.github.io/schemas/wn#domain_region">
    <rdf:type rdf:resource="https://globalwordnet.github.io/schemas/wn#SenseRelType"/>
    <rdfs:comment xml:lang="en">A concept which is a geographical / cultural domain pointer of a given concept.</rdfs:comment>
    <rdfs:comment xml:lang="ja">当該synsetが相手synsetの地域に属するものである</rdfs:comment>
    <rdfs:label xml:lang="en">domain region</rdfs:label>
    <owl:inverseOf rdf:resource="https://globalwordnet.github.io/schemas/wn#has_domain_region"/>
  </SynsetRelType>
  <SynsetRelType rdf:about="https://globalwordnet.github.io/schemas/wn#domain_topic">
    <rdf:type rdf:resource="https://globalwordnet.github.io/schemas/wn#SenseRelType"/>
    <rdfs:comment xml:lang="en">A concept which is the scientific category pointer of a given concept.</rdfs:comment>
    <rdfs:comment xml:lang="ja">当該synsetが相手synsetのカテゴリに属する</rdfs:comment>
    <rdfs:label xml:lang="en">domain topic</rdfs:label>
    <owl:inverseOf rdf:resource="https://globalwordnet.github.io/schemas/wn#has_domain_topic"/>
  </SynsetRelType>
  <SynsetRelType rdf:about="https://globalwordnet.github.io/schemas/wn#entails">
    <rdfs:comment xml:lang="en">impose, involve, or imply as a necessary accompaniment or result</rdfs:comment>
    <rdfs:comment xml:lang="ja">当該synsetを行う場合、必ず相手synsetも行っている</rdfs:comment>
    <rdfs:label xml:lang="en">entails</rdfs:label>
    <owl:inverseOf rdf:resource="https://globalwordnet.github.io/schemas/wn#is_entailed_by"/>
  </SynsetRelType>
  <SynsetRelType rdf:about="https://globalwordnet.github.io/schemas/wn#eq_synonym">
    <rdfs:comment xml:lang="en">X and Y are equivalent concepts but their nature requires that they remain separate (e.g. Exemplifies)</rdfs:comment>
    <rdfs:label xml:lang="en">eq synonym</rdfs:label>
    <owl:inverseOf rdf:resource="https://globalwordnet.github.io/schemas/wn#eq_synonym"/>
  </SynsetRelType>
  <SynsetRelType rdf:about="https://globalwordnet.github.io/schemas/wn#event">
    <rdfs:comment xml:lang="en">An noun representing the event of a verb (e.g., "(a) meet" - "(to) meet")</rdfs:comment>
    <rdfs:label xml:lang="en">event</rdfs:label>
  </SynsetRelType>
  <owl:ObjectProperty rdf:about="https://globalwordnet.github.io/schemas/wn#example">
    <rdfs:comment xml:lang="en">An example usage of a sense or synset</rdfs:comment>
    <rdfs:domain>
      <rdf:Description>
        <owl:unionOf>
          <rdf:Description>
            <rdf:first rdf:resource="http://www.w3.org/ns/lemon/ontolex#LexicalSense"/>
            <rdf:rest>
              <rdf:Description>
                <rdf:first rdf:resource="http://www.w3.org/ns/lemon/ontolex#LexicalConcept"/>
                <rdf:rest rdf:resource="http://www.w3.org/1999/02/22-rdf-syntax-ns#nil"/>
              </rdf:Description>
            </rdf:rest>
          </rdf:Description>
        </owl:unionOf>
      </rdf:Description>
    </rdfs:domain>
    <rdfs:label xml:lang="en">example</rdfs:label>
    <rdfs:range rdf:resource="https://globalwordnet.github.io/schemas/wn#Example"/>
  </owl:ObjectProperty>
  <SynsetRelType rdf:about="https://globalwordnet.github.io/schemas/wn#exemplifies">
    <rdf:type rdf:resource="https://globalwordnet.github.io/schemas/wn#SenseRelType"/>
    <rdfs:comment xml:lang="en">A concept which is the example of a given concept.</rdfs:comment>
    <rdfs:comment xml:lang="ja">当該synsetの用法が相手synsetの領域に限られる</rdfs:comment>
    <rdfs:label xml:lang="en">exemplifies</rdfs:label>
    <owl:inverseOf rdf:resource="https://globalwordnet.github.io/schemas/wn#is_exemplified_by"/>
  </SynsetRelType>
  <SynsetRelType rdf:about="https://globalwordnet.github.io/schemas/wn#feminine">
    <rdfs:comment xml:lang="en">A concept used to refer to female members of a class</rdfs:comment>
    <rdfs:label xml:lang="en">feminine form</rdfs:label>
    <owl:inverseOf rdf:resource="https://globalwordnet.github.io/schemas/wn#has_feminine"/>
  </SynsetRelType>
  <SynsetRelType rdf:about="https://globalwordnet.github.io/schemas/wn#has_augmentative">
    <rdfs:comment xml:lang="en">A concept which has a special concept for generally larger members of its class</rdfs:comment>
    <rdfs:label xml:lang="en">has augmentative form</rdfs:label>
    <owl:inverseOf rdf:resource="https://globalwordnet.github.io/schemas/wn#augmentative"/>
  </SynsetRelType>
  <SynsetRelType rdf:about="https://globalwordnet.github.io/schemas/wn#has_diminutive">
    <rdfs:comment xml:lang="en">A concept which has a special concept for generally smaller members of its class</rdfs:comment>
    <rdfs:label xml:lang="en">has diminutive form</rdfs:label>
    <owl:inverseOf rdf:resource="https://globalwordnet.github.io/schemas/wn#diminutive"/>
  </SynsetRelType>
  <SynsetRelType rdf:about="https://globalwordnet.github.io/schemas/wn#has_domain_region">
    <rdf:type rdf:resource="https://globalwordnet.github.io/schemas/wn#SenseRelType"/>
    <rdfs:comment xml:lang="en">A concept which is the term in the geographical / cultural domain of a given concept.</rdfs:comment>
    <rdfs:comment xml:lang="ja">当該synsetが相手synsetの属する地域である</rdfs:comment>
    <rdfs:label xml:lang="en">has domain region</rdfs:label>
    <owl:inverseOf rdf:resource="https://globalwordnet.github.io/schemas/wn#domain_region"/>
  </SynsetRelType>
  <SynsetRelType rdf:about="https://globalwordnet.github.io/schemas/wn#has_domain_topic">
    <rdf:type rdf:resource="https://globalwordnet.github.io/schemas/wn#SenseRelType"/>
    <rdfs:comment xml:lang="en">A concept which is a term in the scientific category of a given concept.</rdfs:comment>
    <rdfs:comment xml:lang="ja">当該synsetが相手synsetが属するカテゴリである</rdfs:comment>
    <rdfs:label xml:lang="en">has domain topic</rdfs:label>
    <owl:inverseOf rdf:resource="https://globalwordnet.github.io/schemas/wn#domain_topic"/>
  </SynsetRelType>
  <SynsetRelType rdf:about="https://globalwordnet.github.io/schemas/wn#has_feminine">
    <rdfs:comment xml:lang="en">A concept which has a special concept for female members of its class</rdfs:comment>
    <rdfs:label xml:lang="en">has feminine form</rdfs:label>
    <owl:inverseOf rdf:resource="https://globalwordnet.github.io/schemas/wn#feminine"/>
  </SynsetRelType>
  <SynsetRelType rdf:about="https://globalwordnet.github.io/schemas/wn#has_masculine">
    <rdfs:comment xml:lang="en">A concept which has a special concept for male members of its class</rdfs:comment>
    <rdfs:label xml:lang="en">has masculine form</rdfs:label>
    <owl:inverseOf rdf:resource="https://globalwordnet.github.io/schemas/wn#masculine"/>
  </SynsetRelType>
  <SenseRelType rdf:about="https://globalwordnet.github.io/schemas/wn#has_metaphor">
    <rdfs:comment xml:lang="en">a relation between two senses, where the second sense is a metaphorical extension of the first sense</rdfs:comment>
    <rdfs:label xml:lang="en">has metaphor</rdfs:label>
    <owl:inverseOf rdf:resource="https://globalwordnet.github.io/schemas/wn#metaphor"/>
  </SenseRelType>
  <SenseRelType rdf:about="https://globalwordnet.github.io/schemas/wn#has_metonym">
    <rdfs:comment xml:lang="en">a relation between two senses, where the second sense is a metonymical extension of the first sense</rdfs:comment>
    <rdfs:label xml:lang="en">has metonym</rdfs:label>
    <owl:inverseOf rdf:resource="https://globalwordnet.github.io/schemas/wn#metonym"/>
  </SenseRelType>
  <SynsetRelType rdf:about="https://globalwordnet.github.io/schemas/wn#has_young">
    <rdfs:comment xml:lang="en">A concept which has a special concept for young members of its class</rdfs:comment>
    <rdfs:label xml:lang="en">has young form</rdfs:label>
    <owl:inverseOf rdf:resource="https://globalwordnet.github.io/schemas/wn#young"/>
  </SynsetRelType>
  <SynsetRelType rdf:about="https://globalwordnet.github.io/schemas/wn#holo_location">
    <rdfs:comment xml:lang="en">Y is a place located in X</rdfs:comment>
    <rdfs:label xml:lang="en">holonym location</rdfs:label>
    <owl:inverseOf rdf:resource="https://globalwordnet.github.io/schemas/wn#mero_location"/>
  </SynsetRelType>
  <SynsetRelType rdf:about="https://globalwordnet.github.io/schemas/wn#holo_member">
    <rdfs:comment xml:lang="en">Concept B is a member of Concept A</rdfs:comment>
    <rdfs:comment xml:lang="ja">当該synsetが相手synsetという構成員によって構成される</rdfs:comment>
    <rdfs:label xml:lang="en">holonym member</rdfs:label>
    <owl:inverseOf rdf:resource="https://globalwordnet.github.io/schemas/wn#mero_member"/>
  </SynsetRelType>
  <SynsetRelType rdf:about="https://globalwordnet.github.io/schemas/wn#holo_part">
    <rdfs:comment xml:lang="en">Concept B is the whole where Concept A is a part</rdfs:comment>
    <rdfs:comment xml:lang="ja">当該synsetが部分として相手synsetを構成する</rdfs:comment>
    <rdfs:label xml:lang="en">holonym part</rdfs:label>
    <owl:inverseOf rdf:resource="https://globalwordnet.github.io/schemas/wn#mero_part"/>
  </SynsetRelType>
  <SynsetRelType rdf:about="https://globalwordnet.github.io/schemas/wn#holo_portion">
    <rdfs:comment xml:lang="en">Y is an amount/piece/portion of X</rdfs:comment>
    <rdfs:label xml:lang="en">holonym portion</rdfs:label>
    <owl:inverseOf rdf:resource="https://globalwordnet.github.io/schemas/wn#mero_portion"/>
  </SynsetRelType>
  <SynsetRelType rdf:about="https://globalwordnet.github.io/schemas/wn#holo_substance">
    <rdfs:comment xml:lang="en">Concept-B is a substance of Concept-A</rdfs:comment>
    <rdfs:comment xml:lang="ja">当該synsetが相手synsetを構成する物質or材料である</rdfs:comment>
    <rdfs:label xml:lang="en">holonym substance</rdfs:label>
    <owl:inverseOf rdf:resource="https://globalwordnet.github.io/schemas/wn#mero_substance"/>
  </SynsetRelType>
  <SynsetRelType rdf:about="https://globalwordnet.github.io/schemas/wn#holonym">
    <rdfs:comment xml:lang="en">X makes up a part of Y</rdfs:comment>
    <rdfs:comment xml:lang="ja">当該synsetがsynsetを構成する</rdfs:comment>
    <rdfs:label xml:lang="en">holonym</rdfs:label>
    <owl:inverseOf rdf:resource="https://globalwordnet.github.io/schemas/wn#meronym"/>
  </SynsetRelType>
  <SynsetRelType rdf:about="https://globalwordnet.github.io/schemas/wn#hypernym">
    <rdfs:comment xml:lang="pl">Relacja łącząca znaczenie z drugim, ogólniejszym, niż to pierwsze, ale
należącym do tej samej części mowy, co ono</rdfs:comment>
    <rdfs:comment xml:lang="en">a word that is more general than a given word</rdfs:comment>
    <rdfs:label xml:lang="en">hypernym</rdfs:label>
    <rdfs:subPropertyOf rdf:resource="http://www.w3.org/2004/02/skos/core#broader"/>
    <owl:inverseOf rdf:resource="https://globalwordnet.github.io/schemas/wn#hyponym"/>
  </SynsetRelType>
  <SynsetRelType rdf:about="https://globalwordnet.github.io/schemas/wn#hyponym">
    <rdfs:comment xml:lang="en">a word that is more specific than a given word</rdfs:comment>
    <rdfs:comment xml:lang="ja">当該synsetが相手synsetを包含する</rdfs:comment>
    <rdfs:label xml:lang="en">hyponym</rdfs:label>
    <rdfs:subPropertyOf rdf:resource="http://www.w3.org/2004/02/skos/core#narrower"/>
    <owl:inverseOf rdf:resource="https://globalwordnet.github.io/schemas/wn#hypernym"/>
  </SynsetRelType>
  <owl:ObjectProperty rdf:about="https://globalwordnet.github.io/schemas/wn#ili">
    <rdfs:comment xml:lang="en">links a synset to a target the Interlingual Index</rdfs:comment>
    <rdfs:label xml:lang="en">interlingual index</rdfs:label>
    <rdfs:subPropertyOf rdf:resource="http://www.w3.org/2004/02/skos/core#exactMatch"/>
  </owl:ObjectProperty>
  <owl:ObjectProperty rdf:about="https://globalwordnet.github.io/schemas/wn#iliDefinition">
    <rdfs:comment xml:lang="en">The English standard definition of the synset in the ILI</rdfs:comment>
    <rdfs:domain rdf:resource="http://www.w3.org/ns/lemon/ontolex#LexicalConcept"/>
    <rdfs:label xml:lang="en">ILI definition</rdfs:label>
    <rdfs:range rdf:resource="https://globalwordnet.github.io/schemas/wn#ILIDefinition"/>
  </owl:ObjectProperty>
  <SynsetRelType rdf:about="https://globalwordnet.github.io/schemas/wn#in_manner">
    <rdfs:comment xml:lang="en">Y qualifies the manner in which an action or event expressed by X takes place</rdfs:comment>
    <rdfs:label xml:lang="en">in manner</rdfs:label>
    <owl:inverseOf rdf:resource="https://globalwordnet.github.io/schemas/wn#manner_of"/>
  </SynsetRelType>
  <owl:DatatypeProperty rdf:about="https://globalwordnet.github.io/schemas/wn#index">
    <rdfs:comment xml:lang="en">The normalized form of a lexical entry for indexing purposes</rdfs:comment>
    <rdfs:domain rdf:resource="http://www.w3.org/ns/lemon/ontolex#LexicalEntry"/>
    <rdfs:label xml:lang="en">index</rdfs:label>
    <rdfs:range rdf:resource="http://www.w3.org/2000/01/rdf-schema#Literal"/>
  </owl:DatatypeProperty>
  <SynsetRelType rdf:about="https://globalwordnet.github.io/schemas/wn#instance_hypernym">
    <rdfs:comment xml:lang="en">the type of an instance</rdfs:comment>
    <rdfs:comment xml:lang="ja">当該synsetは相手synsetを事例として持つ</rdfs:comment>
    <rdfs:label xml:lang="en">instance hypernym</rdfs:label>
    <owl:inverseOf rdf:resource="https://globalwordnet.github.io/schemas/wn#instance_hyponym"/>
  </SynsetRelType>
  <SynsetRelType rdf:about="https://globalwordnet.github.io/schemas/wn#instance_hyponym">
    <rdfs:comment xml:lang="en">an occurrence of something</rdfs:comment>
    <rdfs:comment xml:lang="ja">当該synsetは相手synsetの事例である</rdfs:comment>
    <rdfs:label xml:lang="en">instance hyponym</rdfs:label>
    <owl:inverseOf rdf:resource="https://globalwordnet.github.io/schemas/wn#instance_hypernym"/>
  </SynsetRelType>
  <SynsetRelType rdf:about="https://globalwordnet.github.io/schemas/wn#instrument">
    <rdf:type rdf:resource="https://globalwordnet.github.io/schemas/wn#SynsetRelType"/>
    <rdfs:comment xml:lang="en">A concept which is the instrument necessary for the action or event expressed by a given concept.</rdfs:comment>
    <rdfs:comment xml:lang="en">An instrument for doing a task (e.g., "photocopier" - "photocopy")</rdfs:comment>
    <rdfs:label xml:lang="en">instrument</rdfs:label>
    <owl:inverseOf rdf:resource="https://globalwordnet.github.io/schemas/wn#involved_instrument"/>
  </SynsetRelType>
  <SynsetRelType rdf:about="https://globalwordnet.github.io/schemas/wn#involved">
    <rdfs:comment xml:lang="en">A concept which is the action or event a given concept typically involved in.</rdfs:comment>
    <rdfs:label xml:lang="en">involved</rdfs:label>
    <owl:inverseOf rdf:resource="https://globalwordnet.github.io/schemas/wn#role"/>
  </SynsetRelType>
  <SynsetRelType rdf:about="https://globalwordnet.github.io/schemas/wn#involved_agent">
    <rdfs:comment xml:lang="en">A concept which is the action done by an agent expressed by a given concept.</rdfs:comment>
    <rdfs:label xml:lang="en">involved agent</rdfs:label>
    <owl:inverseOf rdf:resource="https://globalwordnet.github.io/schemas/wn#agent"/>
  </SynsetRelType>
  <SynsetRelType rdf:about="https://globalwordnet.github.io/schemas/wn#involved_direction">
    <rdfs:comment xml:lang="en">A concept which is the action with the direction expressed by a given concept.</rdfs:comment>
    <rdfs:label xml:lang="en">involved direction</rdfs:label>
    <owl:inverseOf rdf:resource="https://globalwordnet.github.io/schemas/wn#direction"/>
  </SynsetRelType>
  <SynsetRelType rdf:about="https://globalwordnet.github.io/schemas/wn#involved_instrument">
    <rdfs:comment xml:lang="en">A concept which is typically the action with the instrument expressed by a given concept.</rdfs:comment>
    <rdfs:label xml:lang="en">involved instrument</rdfs:label>
    <owl:inverseOf rdf:resource="https://globalwordnet.github.io/schemas/wn#instrument"/>
  </SynsetRelType>
  <SynsetRelType rdf:about="https://globalwordnet.github.io/schemas/wn#involved_location">
    <rdfs:comment xml:lang="en">A concept which is the event happening in a place expressed by a given concept.</rdfs:comment>
    <rdfs:label xml:lang="en">involved location</rdfs:label>
    <owl:inverseOf rdf:resource="https://globalwordnet.github.io/schemas/wn#location"/>
  </SynsetRelType>
  <SynsetRelType rdf:about="https://globalwordnet.github.io/schemas/wn#involved_patient">
    <rdfs:comment xml:lang="en">A concept which is the action that the patient expressed by a given concept undergoing.</rdfs:comment>
    <rdfs:label xml:lang="en">involved patient</rdfs:label>
    <owl:inverseOf rdf:resource="https://globalwordnet.github.io/schemas/wn#patient"/>
  </SynsetRelType>
  <SynsetRelType rdf:about="https://globalwordnet.github.io/schemas/wn#involved_result">
    <rdfs:comment xml:lang="en">A concept which is the action or event with a result of a given concept comes into existence.</rdfs:comment>
    <rdfs:label xml:lang="en">involved result</rdfs:label>
    <owl:inverseOf rdf:resource="https://globalwordnet.github.io/schemas/wn#result"/>
  </SynsetRelType>
  <SynsetRelType rdf:about="https://globalwordnet.github.io/schemas/wn#involved_source_direction">
    <rdfs:comment xml:lang="en">A concept which is the action beginning from a place of a given concept.</rdfs:comment>
    <rdfs:label xml:lang="en">involved source direction</rdfs:label>
    <owl:inverseOf rdf:resource="https://globalwordnet.github.io/schemas/wn#source_direction"/>
  </SynsetRelType>
  <SynsetRelType rdf:about="https://globalwordnet.github.io/schemas/wn#involved_target_direction">
    <rdfs:comment xml:lang="en">A concept which is the action or event leading to a place expressed by a given concept.</rdfs:comment>
    <rdfs:label xml:lang="en">involved target direction</rdfs:label>
    <owl:inverseOf rdf:resource="https://globalwordnet.github.io/schemas/wn#target_direction"/>
  </SynsetRelType>
  <SynsetRelType rdf:about="https://globalwordnet.github.io/schemas/wn#ir_synonym">
    <rdfs:comment xml:lang="en">A concept that means the same except for the style or connotation</rdfs:comment>
    <rdfs:label xml:lang="en">inter-registry synonym</rdfs:label>
    <owl:inverseOf rdf:resource="https://globalwordnet.github.io/schemas/wn#ir_synonym"/>
  </SynsetRelType>
  <SynsetRelType rdf:about="https://globalwordnet.github.io/schemas/wn#is_caused_by">
    <rdfs:comment xml:lang="en">X comes about because of Y</rdfs:comment>
    <rdfs:label xml:lang="en">is caused by</rdfs:label>
    <owl:inverseOf rdf:resource="https://globalwordnet.github.io/schemas/wn#causes"/>
  </SynsetRelType>
  <SynsetRelType rdf:about="https://globalwordnet.github.io/schemas/wn#is_entailed_by">
    <rdfs:comment xml:lang="en">Opposite of entails</rdfs:comment>
    <rdfs:label xml:lang="en">is entailed by</rdfs:label>
    <owl:inverseOf rdf:resource="https://globalwordnet.github.io/schemas/wn#entails"/>
  </SynsetRelType>
  <SynsetRelType rdf:about="https://globalwordnet.github.io/schemas/wn#is_exemplified_by">
    <rdf:type rdf:resource="https://globalwordnet.github.io/schemas/wn#SenseRelType"/>
    <rdfs:comment xml:lang="en">A concept which is the type of a given concept.</rdfs:comment>
    <rdfs:comment xml:lang="ja">当該synsetの領域が相手synsetの用法を規定する</rdfs:comment>
    <rdfs:label xml:lang="en">is exemplified by</rdfs:label>
    <owl:inverseOf rdf:resource="https://globalwordnet.github.io/schemas/wn#exemplifies"/>
  </SynsetRelType>
  <SynsetRelType rdf:about="https://globalwordnet.github.io/schemas/wn#is_subevent_of">
    <rdfs:comment xml:lang="en">X takes place during or as part of Y, and whenever X takes place, Y takes place</rdfs:comment>
    <rdfs:label xml:lang="en">is subevent of</rdfs:label>
    <owl:inverseOf rdf:resource="https://globalwordnet.github.io/schemas/wn#subevent"/>
  </SynsetRelType>
  <owl:DatatypeProperty rdf:about="https://globalwordnet.github.io/schemas/wn#lexfile">
    <rdfs:comments xml:lang="en">Indicates the lexicographer file that this synset is derived from</rdfs:comments>
    <rdfs:label xml:lang="en">lexicographer file</rdfs:label>
  </owl:DatatypeProperty>
  <SynsetRelType rdf:about="https://globalwordnet.github.io/schemas/wn#location">
    <rdf:type rdf:resource="https://globalwordnet.github.io/schemas/wn#SynsetRelType"/>
    <rdfs:comment xml:lang="en">A concept which is the place where the event expressed by a given concept happens.</rdfs:comment>
    <rdfs:comment xml:lang="en">A verb derived from the action performed at a place (e.g., "(a) forge" - "(to) forge")</rdfs:comment>
    <rdfs:label xml:lang="en">location</rdfs:label>
    <owl:inverseOf rdf:resource="https://globalwordnet.github.io/schemas/wn#involved_location"/>
  </SynsetRelType>
  <SynsetRelType rdf:about="https://globalwordnet.github.io/schemas/wn#manner_of">
    <rdfs:comment xml:lang="en">X qualifies the manner in which an action or event expressed by Y takes place</rdfs:comment>
    <rdfs:label xml:lang="en">manner of</rdfs:label>
    <owl:inverseOf rdf:resource="https://globalwordnet.github.io/schemas/wn#in_manner"/>
  </SynsetRelType>
  <SynsetRelType rdf:about="https://globalwordnet.github.io/schemas/wn#masculine">
    <rdfs:comment xml:lang="en">A concept used to refer to male members of a class</rdfs:comment>
    <rdfs:label xml:lang="en">masculine form</rdfs:label>
    <owl:inverseOf rdf:resource="https://globalwordnet.github.io/schemas/wn#has_masculine"/>
  </SynsetRelType>
  <SynsetRelType rdf:about="https://globalwordnet.github.io/schemas/wn#material">
    <rdfs:comment xml:lang="en">A word which is typically the material of a given word (e.g. "wood")</rdfs:comment>
    <rdfs:label xml:lang="en">material</rdfs:label>
  </SynsetRelType>
  <owl:ObjectProperty rdf:about="https://globalwordnet.github.io/schemas/wn#memberList">
    <rdfs:comment xml:lang="en">The list of words in a synset in order</rdfs:comment>
  </owl:ObjectProperty>
  <SynsetRelType rdf:about="https://globalwordnet.github.io/schemas/wn#mero_location">
    <rdfs:comment xml:lang="en">X is a place located in Y</rdfs:comment>
    <rdfs:label xml:lang="en">meronym location</rdfs:label>
    <owl:inverseOf rdf:resource="https://globalwordnet.github.io/schemas/wn#holo_location"/>
  </SynsetRelType>
  <SynsetRelType rdf:about="https://globalwordnet.github.io/schemas/wn#mero_member">
    <rdfs:comment xml:lang="en">Concept A is a member of Concept B</rdfs:comment>
    <rdfs:comment xml:lang="ja">当該synsetが相手synsetの構成員である</rdfs:comment>
    <rdfs:label xml:lang="en">meronym member</rdfs:label>
    <owl:inverseOf rdf:resource="https://globalwordnet.github.io/schemas/wn#holo_member"/>
  </SynsetRelType>
  <SynsetRelType rdf:about="https://globalwordnet.github.io/schemas/wn#mero_part">
    <rdfs:comment xml:lang="en">concept A is a component of concept B</rdfs:comment>
    <rdfs:comment xml:lang="ja">当該synsetが相手synsetという部分によって構成される</rdfs:comment>
    <rdfs:label xml:lang="en">meronym part</rdfs:label>
    <owl:inverseOf rdf:resource="https://globalwordnet.github.io/schemas/wn#holo_part"/>
  </SynsetRelType>
  <SynsetRelType rdf:about="https://globalwordnet.github.io/schemas/wn#mero_portion">
    <rdfs:comment xml:lang="en">X is an amount/piece/portion of Y</rdfs:comment>
    <rdfs:label xml:lang="en">meronym portion</rdfs:label>
    <owl:inverseOf rdf:resource="https://globalwordnet.github.io/schemas/wn#holo_portion"/>
  </SynsetRelType>
  <SynsetRelType rdf:about="https://globalwordnet.github.io/schemas/wn#mero_substance">
    <rdfs:comment xml:lang="en">Concept A is made of concept B.</rdfs:comment>
    <rdfs:comment xml:lang="ja">当該synsetが相手synsetという物質or材料によって構成される</rdfs:comment>
    <rdfs:label xml:lang="en">meronym substance</rdfs:label>
    <owl:inverseOf rdf:resource="https://globalwordnet.github.io/schemas/wn#holo_substance"/>
  </SynsetRelType>
  <SynsetRelType rdf:about="https://globalwordnet.github.io/schemas/wn#meronym">
    <rdfs:comment xml:lang="en">Y makes up a part of X</rdfs:comment>
    <rdfs:comment xml:lang="ja">当該synsetが相手synsetによって構成される</rdfs:comment>
    <rdfs:label xml:lang="en">meronym</rdfs:label>
    <owl:inverseOf rdf:resource="https://globalwordnet.github.io/schemas/wn#holonym"/>
  </SynsetRelType>
  <SenseRelType rdf:about="https://globalwordnet.github.io/schemas/wn#metaphor">
    <rdfs:comment xml:lang="en">a relation between two senses, where the first sense is a metaphorical extension of the second sense</rdfs:comment>
    <rdfs:label xml:lang="en">metaphor</rdfs:label>
    <owl:inverseOf rdf:resource="https://globalwordnet.github.io/schemas/wn#has_metaphor"/>
  </SenseRelType>
  <SenseRelType rdf:about="https://globalwordnet.github.io/schemas/wn#metonym">
    <rdfs:comment xml:lang="en">a relation between two senses, where the first sense is a metonymical extension of the second sense</rdfs:comment>
    <rdfs:label xml:lang="en">metonym</rdfs:label>
    <owl:inverseOf rdf:resource="https://globalwordnet.github.io/schemas/wn#has_metonym"/>
  </SenseRelType>
  <owl:DatatypeProperty rdf:about="https://globalwordnet.github.io/schemas/wn#n">
    <rdfs:comment xml:lang="en">The ordering of a sense within a lexical entry or a normalized group of entries</rdfs:comment>
    <rdfs:domain rdf:resource="http://www.w3.org/ns/lemon/ontolex#LexicalSense"/>
    <rdfs:label xml:lang="en">n</rdfs:label>
    <rdfs:range rdf:resource="http://www.w3.org/2001/XMLSchema#integer"/>
  </owl:DatatypeProperty>
  <PartOfSpeech rdf:about="https://globalwordnet.github.io/schemas/wn#named_entity">
    <rdfs:label xml:lang="en">named entity</rdfs:label>
  </PartOfSpeech>
  <owl:DatatypeProperty rdf:about="https://globalwordnet.github.io/schemas/wn#notation">
    <rdfs:comment xml:lang="en">The notation scheme used for a pronunciation</rdfs:comment>
    <rdfs:domain rdf:resource="https://globalwordnet.github.io/schemas/wn#Pronunciation"/>
    <rdfs:label xml:lang="en">notation</rdfs:label>
  </owl:DatatypeProperty>
  <owl:AnnotationPropety rdf:about="https://globalwordnet.github.io/schemas/wn#note">
    <rdfs:comment xml:lang="en">Any extra notes made by a WordNet creator</rdfs:comment>
    <rdfs:label xml:lang="en">note</rdfs:label>
    <rdfs:range rdf:resource="http://www.w3.org/2001/XMLSchema#string"/>
  </owl:AnnotationPropety>
  <PartOfSpeech rdf:about="https://globalwordnet.github.io/schemas/wn#noun">
    <rdfs:label xml:lang="en">noun</rdfs:label>
    <owl:sameAs rdf:resource="http://www.lexinfo.net/ontology/3.0/lexinfo#noun"/>
  </PartOfSpeech>
  <SynsetRelType rdf:about="https://globalwordnet.github.io/schemas/wn#other">
    <rdf:type rdf:resource="https://globalwordnet.github.io/schemas/wn#SenseRelType"/>
    <rdfs:comment xml:lang="en">Any relation not otherwise specified</rdfs:comment>
    <rdfs:label xml:lang="en">other</rdfs:label>
  </SynsetRelType>
  <PartOfSpeech rdf:about="https://globalwordnet.github.io/schemas/wn#other_pos">
    <rdfs:label xml:lang="en">other pos</rdfs:label>
  </PartOfSpeech>
  <owl:ObjectProperty rdf:about="https://globalwordnet.github.io/schemas/wn#partOfSpeech">
    <rdfs:comment xml:lang="en">The syntactic class of the entry, e.g., noun, verb</rdfs:comment>
    <rdfs:domain>
      <rdf:Description>
        <owl:unionOf>
          <rdf:Description>
            <rdf:first rdf:resource="http://www.w3.org/ns/lemon/ontolex#LexicalEntry"/>
            <rdf:rest>
              <rdf:Description>
                <rdf:first rdf:resource="http://www.w3.org/ns/lemon/ontolex#LexicalConcept"/>
                <rdf:rest rdf:resource="http://www.w3.org/1999/02/22-rdf-syntax-ns#nil"/>
              </rdf:Description>
            </rdf:rest>
          </rdf:Description>
        </owl:unionOf>
      </rdf:Description>
    </rdfs:domain>
    <rdfs:label xml:lang="en">part of speech</rdfs:label>
    <rdfs:range rdf:resource="https://globalwordnet.github.io/schemas/wn#PartOfSpeech"/>
    <rdfs:subPropertyOf rdf:resource="http://www.lexinfo.net/ontology/3.0/lexinfo#partOfSpeech"/>
  </owl:ObjectProperty>
  <SenseRelType rdf:about="https://globalwordnet.github.io/schemas/wn#participle">
    <rdfs:comment xml:lang="en">A concept which is a participial adjective derived from a verb expressed by a given concept.</rdfs:comment>
    <rdfs:label xml:lang="en">participle</rdfs:label>
  </SenseRelType>
  <SynsetRelType rdf:about="https://globalwordnet.github.io/schemas/wn#patient">
    <rdfs:comment xml:lang="en">A concept which is the one/that who/which undergoes a given concept.</rdfs:comment>
    <rdfs:label xml:lang="en">patient</rdfs:label>
    <owl:inverseOf rdf:resource="https://globalwordnet.github.io/schemas/wn#involved_patient"/>
  </SynsetRelType>
  <SenseRelType rdf:about="https://globalwordnet.github.io/schemas/wn#pertainym">
    <rdfs:comment xml:lang="en">A concept which is of or pertaining to a given concept.</rdfs:comment>
    <rdfs:label xml:lang="en">pertainym</rdfs:label>
  </SenseRelType>
  <owl:DatatypeProperty rdf:about="https://globalwordnet.github.io/schemas/wn#phonemic">
    <rdfs:comment xml:lang="en">Indicates if the pronunciation is phonemic, in that it does not represent every aspect of the pronunciation and omits information that could be assumed for this language</rdfs:comment>
    <rdfs:domain rdf:resource="https://globalwordnet.github.io/schemas/wn#Pronunciation"/>
    <rdfs:label xml:lang="en">phonemic</rdfs:label>
  </owl:DatatypeProperty>
  <owl:ObjectProperty rdf:about="https://globalwordnet.github.io/schemas/wn#pronunciation">
    <rdfs:comment xml:lang="en">Indicates the pronunciation of a form</rdfs:comment>
    <rdfs:domain rdf:resource="http://www.w3.org/ns/lemon/ontolex#Form"/>
    <rdfs:label xml:lang="en">pronunciation</rdfs:label>
    <rdfs:range rdf:resource="https://globalwordnet.github.io/schemas/wn#Pronunciation"/>
  </owl:ObjectProperty>
  <SynsetRelType rdf:about="https://globalwordnet.github.io/schemas/wn#property">
    <rdfs:comment xml:lang="en">Cause something to have a particular property (e.g., "magnetize" - "magnetization")</rdfs:comment>
    <rdfs:label xml:lang="en">property</rdfs:label>
  </SynsetRelType>
  <SynsetRelType rdf:about="https://globalwordnet.github.io/schemas/wn#restricted_by">
    <rdfs:comment xml:lang="en">A relation between nominal (pronominal) Y and an adjectival X (quantifier/determiner)</rdfs:comment>
    <rdfs:label xml:lang="en">restricted by</rdfs:label>
    <owl:inverseOf rdf:resource="https://globalwordnet.github.io/schemas/wn#restricts"/>
  </SynsetRelType>
  <SynsetRelType rdf:about="https://globalwordnet.github.io/schemas/wn#restricts">
    <rdfs:comment xml:lang="en">A relation between an adjectival X (quantifier/determiner) and a nominal (pronominal) Y</rdfs:comment>
    <rdfs:label xml:lang="en">restricts</rdfs:label>
    <owl:inverseOf rdf:resource="https://globalwordnet.github.io/schemas/wn#restricted_by"/>
  </SynsetRelType>
  <SynsetRelType rdf:about="https://globalwordnet.github.io/schemas/wn#result">
    <rdf:type rdf:resource="https://globalwordnet.github.io/schemas/wn#SynsetRelType"/>
    <rdfs:comment xml:lang="en">A concept which comes into existence as a result of a given concept.</rdfs:comment>
    <rdfs:comment xml:lang="en">A word which is typically the result of a given word (e.g. "nitrify" - "nitrate")</rdfs:comment>
    <rdfs:label xml:lang="en">result</rdfs:label>
    <owl:inverseOf rdf:resource="https://globalwordnet.github.io/schemas/wn#involved_result"/>
  </SynsetRelType>
  <SynsetRelType rdf:about="https://globalwordnet.github.io/schemas/wn#role">
    <rdfs:comment xml:lang="en">A concept which is involved in the action or event expressed by a given concept.</rdfs:comment>
    <rdfs:label xml:lang="en">role</rdfs:label>
    <owl:inverseOf rdf:resource="https://globalwordnet.github.io/schemas/wn#involved"/>
  </SynsetRelType>
  <owl:DatatypeProperty rdf:about="https://globalwordnet.github.io/schemas/wn#script">
    <rdfs:comment xml:lang="en">The script as a 4 letter ISO 15924 code</rdfs:comment>
    <rdfs:domain rdf:resource="http://www.w3.org/ns/lemon/ontolex#Form"/>
    <rdfs:label xml:lang="en">script</rdfs:label>
    <rdfs:range rdf:resource="http://www.w3.org/2001/XMLSchema#string"/>
  </owl:DatatypeProperty>
  <SynsetRelType rdf:about="https://globalwordnet.github.io/schemas/wn#secondary_aspect_ip">
    <rdfs:comment xml:lang="en">A concept which is linked to another through a change in aspect (ip)</rdfs:comment>
    <rdfs:label xml:lang="en">secondary aspect (imperfect to perfect)</rdfs:label>
    <owl:inverseOf rdf:resource="https://globalwordnet.github.io/schemas/wn#secondary_aspect_pi"/>
  </SynsetRelType>
  <SynsetRelType rdf:about="https://globalwordnet.github.io/schemas/wn#secondary_aspect_pi">
    <rdfs:comment xml:lang="en">A concept which is linked to another through a change in aspect (pi)</rdfs:comment>
    <rdfs:label xml:lang="en">secondary aspect (perfect to imperfect)</rdfs:label>
    <owl:inverseOf rdf:resource="https://globalwordnet.github.io/schemas/wn#secondary_aspect_ip"/>
  </SynsetRelType>
  <owl:ObjectProperty rdf:about="https://globalwordnet.github.io/schemas/wn#senseSubcat">
    <rdfs:comment xml:lang="en">Indicates that a syntactic behaviour applies to a specific sense</rdfs:comment>
    <rdfs:domain rdf:resource="http://www.w3.org/ns/lemon/synsem#SyntacticBehaviour"/>
    <rdfs:label xml:lang="en">sense subcategorization</rdfs:label>
    <rdfs:range rdf:resource="http://www.w3.org/ns/lemon/ontolex#LexicalSense"/>
  </owl:ObjectProperty>
  <SynsetRelType rdf:about="https://globalwordnet.github.io/schemas/wn#similar">
    <rdf:type rdf:resource="https://globalwordnet.github.io/schemas/wn#SenseRelType"/>
    <rdfs:comment xml:lang="en">(of words) expressing closely related meanings</rdfs:comment>
    <rdfs:comment xml:lang="ja">当該synsetは表す意味が相手synsetと近似している</rdfs:comment>
    <rdfs:label xml:lang="en">similar</rdfs:label>
    <owl:inverseOf rdf:resource="https://globalwordnet.github.io/schemas/wn#similar"/>
  </SynsetRelType>
  <SynsetRelType rdf:about="https://globalwordnet.github.io/schemas/wn#simple_aspect_ip">
    <rdfs:comment xml:lang="en">A concept which is linked to another through a change from imperfective to perfective aspect</rdfs:comment>
    <rdfs:label xml:lang="en">simple aspect (imperfect to perfect)</rdfs:label>
    <owl:inverseOf rdf:resource="https://globalwordnet.github.io/schemas/wn#simple_aspect_pi"/>
  </SynsetRelType>
  <SynsetRelType rdf:about="https://globalwordnet.github.io/schemas/wn#simple_aspect_pi">
    <rdfs:comment xml:lang="en">A concept which is linked to another through a change from perfective to imperfective aspect</rdfs:comment>
    <rdfs:label xml:lang="en">simple aspect (perfect to imperfect)</rdfs:label>
    <owl:inverseOf rdf:resource="https://globalwordnet.github.io/schemas/wn#simple_aspect_ip"/>
  </SynsetRelType>
  <owl:ObjectProperty rdf:about="https://globalwordnet.github.io/schemas/wn#sourceSense">
    <rdfs:comment xml:lang="en">The sense that was originally used to define the concept</rdfs:comment>
    <rdfs:domain rdf:resource="https://globalwordnet.github.io/schemas/wn#Definition"/>
    <rdfs:label xml:lang="en">source sense</rdfs:label>
    <rdfs:range rdf:resource="http://www.w3.org/ns/lemon/ontolex#LexicalSense"/>
  </owl:ObjectProperty>
  <SynsetRelType rdf:about="https://globalwordnet.github.io/schemas/wn#source_direction">
    <rdfs:comment xml:lang="en">A concept which is the place from where the event expressed by a given concept begins.</rdfs:comment>
    <rdfs:label xml:lang="en">source direction</rdfs:label>
    <owl:inverseOf rdf:resource="https://globalwordnet.github.io/schemas/wn#involved_source_direction"/>
  </SynsetRelType>
  <SynsetRelType rdf:about="https://globalwordnet.github.io/schemas/wn#state">
    <rdfs:comment xml:lang="en">A state caused by the verb (e.g., "sensitize" - "sensitization")</rdfs:comment>
    <rdfs:label xml:lang="en">state</rdfs:label>
  </SynsetRelType>
  <SynsetRelType rdf:about="https://globalwordnet.github.io/schemas/wn#state_of">
    <rdfs:comment xml:lang="en">Y is qualified by X</rdfs:comment>
    <rdfs:label xml:lang="en">state of</rdfs:label>
    <owl:inverseOf rdf:resource="https://globalwordnet.github.io/schemas/wn#be_in_state"/>
  </SynsetRelType>
  <owl:AnnotationProperty rdf:about="https://globalwordnet.github.io/schemas/wn#status">
    <rdfs:comment xml:lang="en">A status string such as, 'finalized', 'checked' or 'to check'</rdfs:comment>
    <rdfs:label xml:lang="en">status</rdfs:label>
    <rdfs:range rdf:resource="http://www.w3.org/2001/XMLSchema#string"/>
  </owl:AnnotationProperty>
  <SynsetRelType rdf:about="https://globalwordnet.github.io/schemas/wn#subevent">
    <rdfs:comment xml:lang="en">Y takes place during or as part of X, and whenever Y takes place, X takes place</rdfs:comment>
    <rdfs:label xml:lang="en">subevent</rdfs:label>
    <owl:inverseOf rdf:resource="https://globalwordnet.github.io/schemas/wn#is_subevent_of"/>
  </SynsetRelType>
  <owl:ObjectProperty rdf:about="https://globalwordnet.github.io/schemas/wn#tag">
    <rdfs:comment xml:lang="en">A tag describing an inflected form. There are no specific guidelines about the form of this element</rdfs:comment>
    <rdfs:domain rdf:resource="http://www.w3.org/ns/lemon/ontolex#Form"/>
    <rdfs:label xml:lang="en">tag</rdfs:label>
    <rdfs:range rdf:resource="https://globalwordnet.github.io/schemas/wn#Tag"/>
  </owl:ObjectProperty>
  <SynsetRelType rdf:about="https://globalwordnet.github.io/schemas/wn#target_direction">
    <rdfs:comment xml:lang="en">A concept which is the place where the action or event expressed by a given concept leads to.</rdfs:comment>
    <rdfs:label xml:lang="en">target direction</rdfs:label>
    <owl:inverseOf rdf:resource="https://globalwordnet.github.io/schemas/wn#involved_target_direction"/>
  </SynsetRelType>
  <SynsetRelType rdf:about="https://globalwordnet.github.io/schemas/wn#undergoer">
    <rdfs:comment xml:lang="en">A word which is typically the undergoer of a given word (e.g. "honor" - "honoree")</rdfs:comment>
    <rdfs:label xml:lang="en">undergoer</rdfs:label>
  </SynsetRelType>
  <PartOfSpeech rdf:about="https://globalwordnet.github.io/schemas/wn#unknown_pos">
    <rdfs:label xml:lang="en">unknown pos</rdfs:label>
  </PartOfSpeech>
  <SynsetRelType rdf:about="https://globalwordnet.github.io/schemas/wn#uses">
    <rdfs:comment xml:lang="en">A verb that uses a noun (e.g., "(to) talc" - "talc")</rdfs:comment>
    <rdfs:label xml:lang="en">uses</rdfs:label>
  </SynsetRelType>
  <owl:DatatypeProperty rdf:about="https://globalwordnet.github.io/schemas/wn#variety">
    <rdfs:comment xml:lang="en">Indicates the variety of language the pronunciation represents</rdfs:comment>
    <rdfs:domain rdf:resource="https://globalwordnet.github.io/schemas/wn#Pronunciation"/>
    <rdfs:label xml:lang="en">variety</rdfs:label>
  </owl:DatatypeProperty>
  <SynsetRelType rdf:about="https://globalwordnet.github.io/schemas/wn#vehicle">
    <rdfs:comment xml:lang="en">A verb indicating movement with a particular vehicle (e.g., "(to) ship" - "ship")</rdfs:comment>
    <rdfs:label xml:lang="en">vehicle</rdfs:label>
  </SynsetRelType>
  <PartOfSpeech rdf:about="https://globalwordnet.github.io/schemas/wn#verb">
    <rdfs:label xml:lang="en">verb</rdfs:label>
    <owl:sameAs rdf:resource="http://www.lexinfo.net/ontology/3.0/lexinfo#verb"/>
  </PartOfSpeech>
  <SynsetRelType rdf:about="https://globalwordnet.github.io/schemas/wn#young">
    <rdfs:comment xml:lang="en">A concept used to refer to young members of a class</rdfs:comment>
    <rdfs:label xml:lang="en">young form</rdfs:label>
    <owl:inverseOf rdf:resource="https://globalwordnet.github.io/schemas/wn#has_young"/>
  </SynsetRelType>
</rdf:RDF>
